@prefix : <https://w3id.org/controverse#> .
@prefix cover: <https://w3id.org/controverse#> .
@prefix owl: <http://www.w3.org/2002/07/owl#> .
@prefix rdfs: <http://www.w3.org/2000/01/rdf-schema#> .
@prefix xsd: <http://www.w3.org/2001/XMLSchema#> .
@prefix creon: <http://www.ontologydesignpatterns.org/ont/creativity/creon.owl#> .
@base <https://w3id.org/controverse#> .


# Ontology: ControVerse (CoVer)

<https://w3id.org/controverse#> rdf:type owl:Ontology ;
                                dc:creator "Fahmida Islam" ,
                                            "Ilaria De Dominicis",
                                            "Regina Manyara";
                                rdfs:comment "An ontology about irony in Lyrical works.";
                                owl:versionInfo "November 2025". # ! put the date of the exam here


# Annotation property 

<http://www.w3.org/ns/prov#wasAttributedTo> rdf:type owl:AnnotationProperty . # now it can have a literal as object 
# ! If Palacio took something from Muecke, then we should say that what she said 'wasDerivedFrom'; see here: https://www.w3.org/ns/prov :D 

# Classes

cover:CreativeWork a owl:Class ;
    owl:equivalentClass creon:CreativeProduct ;
    rdfs:comment "It is something that is produced as a result of the creative process, by a specific Person" .
    
cover:LyricalWork a owl:Class ;
    owl:equivalentClass creon:CreativeDomain ; 
    rdfs:subClassOf cover:CreativeWork ;
    rdfs:comment "A piece of writing, art, or music that is beautifully expressive and emotional, often with a poetic, song-like quality." .

cover:Song a owl:Class ;
    rdfs:subClassOf cover:LyricalWork ;
    rdfs:comment "A short poem or other set of words set to music or meant to be sung." ; <http://www.w3.org/ns/prov#wasAttributedTo> "Oxford Languages" .

cover:Poem a owl:Class ;
    rdfs:subClassOf cover:LyricalWork ;
    rdfs:comment "A piece of writing in which the expression of feelings and ideas is given intensity by particular attention to diction (sometimes involving rhyme), rhythm, and imagery." ;
    <http://www.w3.org/ns/prov#wasAttributedTo> "Oxford Languages" .

cover:Actor a owl:Class ;
    owl:equivalentClass creon:Agent ;
    rdfs:comment "An entity performing an action in an creative context. Includes author, performer, ironist, or interpreter." .

cover:Author a owl:Class ;
    rdfs:subClassOf cover:Actor ;
    rdfs:comment "The creator of the text or composition that doesn't contain irony, but sincerity." .

cover:Ironist a owl:Class ;
    rdfs:subClassOf cover:Author ;
    rdfs:comment "The creator of the text or composition that contains irony." ;
    <http://www.w3.org/ns/prov#wasAttributedTo> "Lozano Palacio, Inés. ‘A Scenario-Based Approach to Irony. Structure, Meaning and Function’. PhD Thesis, 2020." . 

cover:Interpreter a owl:Class ;
    rdfs:subClassOf cover:Actor ;
    rdfs:comment "The one who perceives or decodes irony and makes the Ironic Event possible. It can be a listener or a reader." ;
    <http://www.w3.org/ns/prov#wasAttributedTo> "Lozano Palacio, Inés. ‘A Scenario-Based Approach to Irony. Structure, Meaning and Function’. PhD Thesis, 2020." .   

cover:Reader a owl:Class ;
    rdfs:subClassOf cover:Interpreter ;
    rdfs:comment "The one who is able to decode irony while reading to the Creative Work. " .

cover:Listener a owl:Class ;
    rdfs:subClassOf cover:Interpreter ;
    rdfs:comment "The one who is able to decode irony while listening to the Creative Work. " .

cover:Performer a owl:Class ;
    rdfs:subClassOf cover:Actor ;
    rdfs:comment "The person who performs or stages the Creative work work." .

cover:Target a owl:Class ;
    rdfs:comment "We understand the notion of target as the object of the ironic remark, be it (i) a person, (ii) a state of affairs, (iii) an institution, or (iv) another type of animate or inanimate entity. If the target of the irony is a person, he/she may be either present or absent. (Lozano Palacio, 2020, p. 159)" ;
    <http://www.w3.org/ns/prov#wasAttributedTo> "Lozano Palacio, Inés. ‘A Scenario-Based Approach to Irony. Structure, Meaning and Function’. PhD Thesis, 2020." .

cover:Institution a owl:Class ;
    rdfs:subClassOf cover:Target ;
    rdfs:comment "The collective entity toward which irony is directed." .

cover:Community a owl:Class ;
    rdfs:subClassOf cover:Target ;
    rdfs:comment "The social or cultural entity toward which irony is directed." .

cover:Person a owl:Class ;
    rdfs:subClassOf cover:Target ;
    rdfs:comment "The individual toward which irony is directed." .

cover:Self a owl:Class ;
    rdfs:subClassOf cover:Person ;
    rdfs:comment "The self as the subject or object of irony (self-irony)." .

cover:Concept a owl:Class ;
    rdfs:subClassOf cover:Target ;
    rdfs:comment "The abstract idea or notion toward which irony is directed." .

cover:Thing a owl:Class ;
    rdfs:subClassOf cover:Target ;
    rdfs:comment "The concrete object toward which irony is directed." .

cover:StateOfAffair a owl:Class ;
    rdfs:subClassOf cover:Target ;
    rdfs:comment "The situation or condition toward which irony is directed." .

cover:Event a owl:Class ;
    rdfs:comment "A situation or condition in which irony may or may not arise." .

cover:IronicEvent a owl:Class ;
    rdfs:subClassOf cover:Event ;
    owl:equivalentClass creon:CreativeSituation ;
    rdfs:comment "The situation where the concept of irony arises: there is a clash between the Epistemic and the Observable Scenarios." .

cover:SincereEvent a owl:Class ;
    rdfs:subClassOf cover:Event ;
    rdfs:comment "The situation where the concept of irony does not arise: there is no clash between the Epistemic and the Observable Scenarios.".

cover:EpistemicScenario a owl:Class ;
    rdfs:comment "We define the epistemic scenario as the conceptual correlate of a state of affairs that someone regards as highly likely or certain to occur. (Lozano Palacio, 2020, p. 101)" ;
    <http://www.w3.org/ns/prov#wasAttributedTo> "Lozano Palacio, Inés. ‘A Scenario-Based Approach to Irony. Structure, Meaning and Function’. PhD Thesis, 2020." .

cover:ObservableScenario a owl:Class ;
    rdfs:comment "The observable scenario, both in verbal and situational irony, can be what the ironist and the interpreter perceive, which contradicts their expectations or firm beliefs about a given state of affairs. (Lozano Palacio, 2020, p. 124)" ;
    <http://www.w3.org/ns/prov#wasAttributedTo> "Lozano Palacio, Inés. ‘A Scenario-Based Approach to Irony. Structure, Meaning and Function’. PhD Thesis, 2020." .


cover:ListeningEvent a owl:Class ;
    rdfs:subClassOf cover:Event ;
    rdfs:comment "An event of oral reception (e.g., listening to an ironic song)." .

cover:ReadingEvent a owl:Class ;
    rdfs:subClassOf cover:Event ;
    rdfs:comment "An event of textual reception (e.g., reading an ironic poem)." .

cover:Irony a owl:Class ;
    owl:equivalentClass creon:CreativeIdea ;
    rdfs:comment "The abstract concept of irony." .

cover:Sincerity a owl:Class ;
    owl:equivalentClass creon:CreativeIdea ;
    rdfs:comment "The concept opposite to irony; there is no clash between scenarios." .

cover:VerbalIrony a owl:Class ; 
    rdfs:subClassOf cover:Irony ;
    rdfs:comment "Verbal Irony implies an ironist, someone consciously and intentionally employing a technique. (Muecke, D.C., 2020, p. 42)" ;
    <http://www.w3.org/ns/prov#wasAttributedTo> "Muecke, Douglas Colin. 'The compass of irony'. Routledge Revivals, 2020." .


cover:SituationalIrony a owl:Class ;
    rdfs:subClassOf cover:Irony ;
    rdfs:comment "Situational Irony does not imply an ironist but merely 'a condition of affairs' or 'outcome of events' which, we add, is seen and felt to be ironic. (Muecke, D.C., 2020, p. 42)" ;
    <http://www.w3.org/ns/prov#wasAttributedTo> "Muecke, Douglas Colin. 'The compass of irony'. Routledge Revivals, 2020." .

cover:ImpersonalIrony a owl:Class ;
    rdfs:subClassOf cover:VerbalIrony ;
    rdfs:comment "The irony resides more in what he (the ironist) says than in the fact that it is a man of a particular character saying it.(Muecke, D.C., 2020, p. 61)" ;
    <http://www.w3.org/ns/prov#wasAttributedTo> "Muecke, Douglas Colin. 'The compass of irony'. Routledge Revivals, 2020." .

cover:SelfDisparagingIrony a owl:Class ;
    rdfs:subClassOf cover:VerbalIrony ;
    rdfs:comment "The ironist is present not simply as an impersonal voice but, in disguise, as a person with certain characteristics. And the sort of person the ironist presents himself as being is our guide to his real opinion. He understates or overstates himself, assuming such qualities as ignorance, deference, complaisance, co-operativeness, naivety, over-enthusiasm, eagerness to learn, and inability to understand. But his disguise is meant to be penetrated, and our judgement is directed not against the ignorance or naivety of the speaker but against the object of the irony.(Muecke, D.C., 2020, p. 87)" ;
    <http://www.w3.org/ns/prov#wasAttributedTo> "Muecke, Douglas Colin. 'The compass of irony'. Routledge Revivals, 2020." .

cover:IngenuIrony a owl:Class ;
    rdfs:subClassOf cover:VerbalIrony ;
    rdfs:comment "Ingénu Irony is almost archetypically represented by Hans Andersen's fable, The Emperor's New Clothes. The effectiveness of this kind of irony conies from its economy of means: mere common sense or even simple innocence or ignorance may suffice to see through the woven complexities of hypocrisy and rationalization or pierce the protective tissues of convention and idées revues. The ironist does not need to put forth all his powers. (Muecke, D.C., 2020, p. 91)" ;
    <http://www.w3.org/ns/prov#wasAttributedTo> "Muecke, Douglas Colin. 'The compass of irony'. Routledge Revivals, 2020." .

cover:DramatizedIrony a owl:Class ;
    rdfs:subClassOf cover:VerbalIrony ;
    rdfs:comment "The function of the ironist in Dramatized Irony is simply to present ironic situations or events to our sense of irony. (Ironic situations and events themselves I shall discuss and attempt to classify in the next chapter.) In this ironic mode the ironist does not appear either as an impersonal voice or in any disguise. He simply arranges that the characters of his play or novel, story, verse narrative, or dramatic monologue expose themselves in their ironic predicament directly to the audience or reader. He himself is the puppet-master and as such out of sight. This is the only way in which dramatists can be ironical (short of bringing themselves more or less identifiably on stage). This is the way in which such novelists as Flaubert and Joyce are ironical. Novelists, such as Thackeray, who comment on their characters. (Muecke, D.C., 2020, pp. 92-93)" ;
    <http://www.w3.org/ns/prov#wasAttributedTo> "Muecke, Douglas Colin. 'The compass of irony'. Routledge Revivals, 2020." .

cover:IronyOfSimpleIncongruency a owl:Class ;
    rdfs:subClassOf cover:SituationalIrony ;
    rdfs:comment "Since there is incongruity in all ironic situations, the kind of ironic situation that, for want of any other distinguishing characteristic, appears under this unsatisfactory heading must be regarded as, formally speaking, a sort of minimal irony. It is irony in its barest and simplest terms uncomplicated by the presentation of action or character or the victim's imperception (though, of course, there is an imperception to be inferred). (Muecke, D.C., 2020, p. 100)" ;
    <http://www.w3.org/ns/prov#wasAttributedTo> "Muecke, Douglas Colin. 'The compass of irony'. Routledge Revivals, 2020." .

cover:IronyOfEvents a owl:Class ;
    rdfs:subClassOf cover:SituationalIrony ;
    rdfs:comment "Here the ironic incongruity is between the expectation and the event. We say it is ironic when, after we have more or less explicitly or confidently expressed reliance in the way things go, some subsequent unforeseen turn of events reverses and frustrates our expectations or designs. It is ironic when we meet what we set out to avoid, especially when the means we take to avoid something turn out to be the very means of bringing about what we sought to avoid. It is ironic when we get at last what we no longer desire. (Muecke, D.C., 2020, p. 102)" ;
    <http://www.w3.org/ns/prov#wasAttributedTo> "Muecke, Douglas Colin. 'The compass of irony'. Routledge Revivals, 2020." .

cover:IronyOfDrama a owl:CLass ;
    rdfs:subClassOf cover:SituationalIrony ;
    rdfs:comment "Generally speaking the irony is more striking when an observer already knows what the victim has yet to find out. To the examiner who has already failed the student whom he hears expressing a confident expectation of passing, the situation is already ironic; to others there is no irony until the results come out. (Muecke, D.C., 2020, p. 104)" ;
    <http://www.w3.org/ns/prov#wasAttributedTo> "Muecke, Douglas Colin. 'The compass of irony'. Routledge Revivals, 2020." .

cover:IronyOfSelfBetrayal a owl:Class ;
    rdfs:subClassOf cover:SituationalIrony ;
    rdfs:comment "It is exemplified whenever someone, by what he says or does (not by what happens to him), exposes unawares his own ignorance, weaknesses, errors, or follies [...] The dramatist or novelist who is interested in people will be aware that, in spite of much unexceptionable advice, mankind's progress in self-knowledge has been indifferent; he hath ever but slenderly known himself, and consequently can scarcely open his mouth without betraying himself. (Muecke, D.C., 2020, p. 107)" ;
    <http://www.w3.org/ns/prov#wasAttributedTo> "Muecke, Douglas Colin. 'The compass of irony'. Routledge Revivals, 2020." .

cover:IronyOfDilemma a owl:Class ;
    rdfs:subClassOf cover:SituationalIrony ;
    rdfs:comment "The victim of a dilemma or some other impossible situation may be a victim of an ironic situation in several different ways. He may, for example, be confidently unaware of being so situated. (Muecke, D.C., 2020, p. 113)" ;
    <http://www.w3.org/ns/prov#wasAttributedTo> "Muecke, Douglas Colin. 'The compass of irony'. Routledge Revivals, 2020." .

# Object Properties

cover:hasScenario a owl:ObjectProperty ;
    rdfs:domain cover:CreativeWork ;
    rdfs:range [ a owl:Class ; owl:unionOf (cover:EpistemicScenario cover:ObservableScenario) ] ;
    rdfs:label "has scenario" ;
    rdfs:comment "Links a work or event to the scenario in which irony may occur." .

cover:hasActor a owl:ObjectProperty ;
    rdfs:domain cover:IronicEvent ;
    rdfs:range cover:Actor ;
    rdfs:label "has actor" ;
    rdfs:comment "Any person involved in a Creative Process." .

cover:hasTarget a owl:ObjectProperty ;
    rdfs:domain cover:IronicEvent ;
    rdfs:range cover:Target ;
    rdfs:label "has target" ;
    rdfs:comment "Indicates the target or object of irony." .

cover:hasEvent a owl:ObjectProperty ;
    rdfs:domain cover:IronicEvent ;
    rdfs:range cover:Event ;
    rdfs:label "has event" ;
    rdfs:comment "Connects irony to a specific event (performance, reading, listening)." .

cover:hasLyricalType a owl:ObjectProperty ;
    rdfs:domain cover:CreativeWork ;
    rdfs:range [ a owl:Class ; owl:unionOf (cover:Poem cover:Song) ] ; # ! should they be disjointed?
    rdfs:label "has irony type" ;
    rdfs:comment "Specifies whether irony is Verbal or Situational." .

cover:hasIronyType a owl:ObjectProperty ;
    rdfs:domain cover:Irony ;
    rdfs:range [ a owl:Class ; owl:unionOf (cover:VerbalIrony cover:SituationalIrony) ] ;
    rdfs:label "has irony type" ;
    rdfs:comment "Specifies whether irony is Verbal or Situational." .

cover:hasIronySubtype a owl:ObjectProperty ;
    rdfs:domain cover:Irony ;
    rdfs:range [ a owl:Class ; owl:unionOf (
        cover:DramaticIrony
        cover:ImpersonalIrony
        cover:SelfDisparagingIrony
        cover:IngenuIrony
        cover:IronyOfSimpleIncongruency
        cover:IronyOfSimpleEvents
        cover:IronyOfSelfBetrayal
        cover:IronyOfDilemma ) ] ;
    rdfs:label "has irony subtype" ;
    rdfs:comment "Defines the subtype of irony." .

cover:hasInstance a owl:ObjectProperty ;
    rdfs:domain cover:Event ;
    rdfs:range [ a owl:Class ; owl:unionOf (cover:Irony cover:Sincerity) ] ;
    rdfs:label "has instance" ;
    rdfs:comment "Whether the event is Ironic (clash between Epistemic and Observable Scenarios) or Sincere (no clash between the two scenarios)." .

cover:hasInterpreter a owl:ObjectProperty ;
    rdfs:domain cover:CreativeWork ;
    rdfs:range cover:Interpreter ;
    rdfs:label "has interpreter" ;
    rdfs:comment "Language of the work." .

cover:hasCreator a owl:ObjectProperty ; # creator as Object 
    rdfs:domain cover:CreativeWork ;
    rdfs:range [
        a owl:Class ;
        owl:unionOf ( cover:Author cover:Ironist )
    ] ;
    rdfs:label "has creator" ;
    rdfs:comment "Links a creative work to the one who perceives or decodes irony and makes the Ironic Event possible. It can be a reader or listener" .

cover:hasPerformer a owl:ObjectProperty ; # performer as Object
    rdfs:domain cover:CreativeWork ;
    rdfs:range cover:Performer ;
    rdfs:label "has performer" ;
    rdfs:comment "Links a creative work to the person or entity who performed it." .

# Data Properties

cover:hasCreationDate a owl:DatatypeProperty ;
    rdfs:domain cover:CreativeWork ;
    rdfs:range [
        a rdfs:Datatype ;
        owl:unionOf ( xsd:gYear xsd:string )
    ] ;
    rdfs:label "has creation date" ;
    rdfs:comment "Date when the work was created. Can be expressed as a year or a string." .

cover:hasTitle a owl:DatatypeProperty ;
    rdfs:domain cover:CreativeWork ;
    rdfs:range xsd:string ;
    rdfs:label "has title" ;
    rdfs:comment "Title of the work." .

cover:hasEventLocation a owl:DatatypeProperty ;
    rdfs:domain cover:Event ;
    rdfs:range xsd:string ;
    rdfs:label "has event location" ;
    rdfs:comment "Location where the event took place." .

cover:hasCreationLocation a owl:DatatypeProperty ;
    rdfs:domain cover:CreativeWork ;
    rdfs:range xsd:string ;
    rdfs:label "has creation location" ;
    rdfs:comment "Location where the work was created." .

cover:hasDescription a owl:DatatypeProperty ;
    rdfs:range xsd:string ;
    rdfs:label "has description" ;
    rdfs:comment "Any general description." .

cover:hasLanguage a owl:DatatypeProperty ;
    rdfs:domain cover:CreativeWork ;
    rdfs:range xsd:string ;
    rdfs:label "has language" ;
    rdfs:comment "Language of the work or the instance." .

cover:hasPoeticForm a owl:DatatypeProperty ;
    rdfs:domain cover:CreativeWork ;
    rdfs:range xsd:string ;
    rdfs:label "has poetic form" ;
    rdfs:comment "Specifies the poetic form (e.g., sonnet, ballad, cantata)." .

cover:hasGenre a owl:DatatypeProperty ;
    rdfs:domain cover:CreativeWork ;
    rdfs:range xsd:string ;
    rdfs:label "has genre" ;
    rdfs:comment "Indicates the musical or literary genre." .

cover:hasCreatorName a owl:DatatypeProperty ; # creator as Literal
    rdfs:domain cover:CreativeWork ;
    rdfs:range xsd:string ;
    rdfs:label "has creator name" ;
    rdfs:comment "Indicates the creator of the work as a literal name (string)." .

cover:hasPerformerName a owl:DatatypeProperty ; # performer as Literal
    rdfs:domain cover:CreativeWork ;
    rdfs:range xsd:string ;
    rdfs:label "has performer name" ;
    rdfs:comment "Indicates the performer of the work as a literal name (string)." .

# disjoint Classes

cover:Interpreter owl:disjointWith cover:Author . # int. is never the author of the work...
cover:Interpreter owl:disjointWith cover:Ironist . #... or the ironist
cover:Irony owl:disjointWith cover:Sincerity . 
cover:IronicEvent owl:disjointWith cover:SincereEvent .
